Add invariant to untick-proof

compiler/backend/proofs/thunk_subst_untickProofScript.sml
@@ -93,8 +93,6 @@ Inductive exp_rel:
        v_rel (DoTick v) w)
 End
 
-Theorem SUM_REL_def[simp,local] = quotient_sumTheory.SUM_REL_def;
-
 Theorem exp_rel_subst:
   ∀vs x ws y.
     LIST_REL v_rel (MAP SND vs) (MAP SND ws) ∧
@@ -189,23 +187,211 @@ Proof
   \\ ho_match_mp_tac exp_rel_strongind \\ rw []
 QED
 
+Definition proper_thunk_def[simp]:
+  proper_thunk (Thunk x) = (∃y. x = INR y) ∧
+  proper_thunk (Recclosure f n) =
+    (∃x. ALOOKUP (REVERSE f) n = SOME (Delay x)) ∧
+  proper_thunk _ = F
+End
+
+Theorem proper_thunk_dest_anyThunk:
+  ∀v. proper_thunk v ⇒
+    ∃x ws. dest_anyThunk v = INR (INR x, ws)
+Proof
+  Induct \\ rw [] \\ simp [dest_anyThunk_def]
+QED
+
+Inductive exp_inv:
+[~Var:]
+  (∀n.
+     exp_inv (Var n)) ∧
+[~Value:]
+  (∀v.
+     v_inv v ⇒
+       exp_inv (Value v)) ∧
+[~Prim:]
+  (∀op xs.
+     EVERY exp_inv xs ⇒
+       exp_inv (Prim op xs)) ∧
+[~App:]
+  (∀f x.
+     exp_inv f ∧
+     exp_inv x ⇒
+       exp_inv (App f x)) ∧
+[~Lam:]
+  (∀s x.
+     exp_inv x ⇒
+       exp_inv (Lam s x)) ∧
+[~Letrec:]
+  (∀f x.
+     EVERY exp_inv (MAP SND f) ∧
+     exp_inv x ⇒
+       exp_inv (Letrec f x)) ∧
+[~Let:]
+  (∀s x y.
+     exp_inv x ∧
+     exp_inv y ⇒
+       exp_inv (Let s x y)) ∧
+[~If:]
+  (∀x y z.
+     EVERY exp_inv [x;y;z] ⇒
+       exp_inv (If x y z)) ∧
+[~Delay:]
+  (∀x.
+     exp_inv x ⇒
+        exp_inv (Delay x)) ∧
+[~Box:]
+  (∀x.
+     exp_inv x ⇒
+       exp_inv (Box x)) ∧
+[~Force:]
+  (∀x.
+     exp_inv x ⇒
+       exp_inv (Force x)) ∧
+[~MkTick:]
+  (∀x.
+     exp_inv x ⇒
+       exp_inv (MkTick x)) ∧
+[v_inv_Constructor:]
+  (∀s vs.
+     EVERY v_inv vs ⇒
+       v_inv (Constructor s vs)) ∧
+[v_inv_Closure:]
+  (∀s x.
+     exp_inv x ⇒
+       v_inv (Closure s x)) ∧
+[v_inv_Recclosure:]
+  (∀f n.
+     EVERY exp_inv (MAP SND f) ⇒
+       v_inv (Recclosure f n)) ∧
+[v_inv_Thunk_INR:]
+  (∀x.
+     exp_inv x ⇒
+       v_inv (Thunk (INR x))) ∧
+[v_inv_Thunk_INL:]
+  (∀v.
+     v_inv v ⇒
+       v_inv (Thunk (INL v))) ∧
+[v_inv_Atom:]
+  (∀x.
+     v_inv (Atom x)) ∧
+[v_inv_DoTick:]
+  (∀v.
+     v_inv v ∧
+     proper_thunk v ⇒
+       v_inv (DoTick v))
+End
+
+fun vapply tm =
+  let
+    val ty = List.hd (#1 (strip_fun (type_of tm)))
+             handle Empty => fail()
+    val v = variant (free_vars tm) (mk_var ("x", ty))
+    val tm = mk_comb (tm, v)
+  in
+    vapply tm
+  end
+  handle HOL_ERR _ => tm;
+
+Theorem exp_inv_def =
+  TypeBase.constructors_of “:exp”
+  |> map (curry mk_comb “exp_inv” o vapply)
+  |> map (SIMP_CONV (srw_ss()) [Once exp_inv_cases])
+  |> LIST_CONJ;
+
+Theorem v_inv_def =
+  TypeBase.constructors_of “:v”
+  |> map (curry mk_comb “v_inv” o vapply)
+  |> map (SIMP_CONV (srw_ss()) [Once exp_inv_cases])
+  |> LIST_CONJ;
+
+Theorem SUM_REL_def[simp,local] = quotient_sumTheory.SUM_REL_def;
+
+Theorem exp_inv_subst:
+  ∀vs x.
+    EVERY v_inv (MAP SND vs) ∧
+    exp_inv x ⇒
+      exp_inv (subst vs x)
+Proof
+  ho_match_mp_tac subst_ind \\ rw []
+  >- ((* Var *)
+    gs [exp_inv_def, subst_def, EVERY_MAP, EVERY_EL]
+    \\ CASE_TAC \\ gs [exp_inv_def]
+    \\ drule_then strip_assume_tac ALOOKUP_SOME_REVERSE_EL
+    \\ first_x_assum (drule_then strip_assume_tac) \\ gs [])
+  >- ((* Prim *)
+    gs [exp_inv_def] \\ simp [subst_def]
+    \\ irule exp_inv_Prim
+    \\ gs [EVERY_MAP, EVERY_MEM])
+  >- ((* If *)
+    gs [exp_inv_def] \\ simp [subst_def]
+    \\ irule exp_inv_If \\ fs [])
+  >- ((* App *)
+    gs [exp_inv_def] \\ simp [subst_def]
+    \\ irule exp_inv_App \\ fs [])
+  >- ((* Lam *)
+    gs [exp_inv_def] \\ simp [subst_def]
+    \\ irule exp_inv_Lam
+    \\ first_x_assum irule
+    \\ gs [EVERY_MAP, EVERY_FILTER, LAMBDA_PROD, EVERY_MEM, FORALL_PROD,
+           SF SFY_ss])
+  >- ((* Let NONE *)
+    gs [exp_inv_def] \\ simp [subst_def]
+    \\ irule exp_inv_Let \\ fs [])
+  >- ((* Let SOME *)
+    gs [exp_inv_def] \\ simp [subst_def]
+    \\ irule exp_inv_Let \\ fs []
+    \\ first_x_assum irule
+    \\ gs [EVERY_MAP, EVERY_FILTER, LAMBDA_PROD, EVERY_MEM, FORALL_PROD,
+           SF SFY_ss])
+  >- ((* Letrec *)
+    gs [exp_inv_def] \\ simp [subst_def]
+    \\ irule exp_inv_Letrec
+    \\ gvs [EVERY_MAP, LAMBDA_PROD]
+    \\ first_assum (irule_at Any)
+    \\ gvs [EVERY_FILTER, LAMBDA_PROD]
+    \\ qabbrev_tac ‘P = λx. ¬MEM x (MAP FST f)’ \\ fs []
+    \\ irule_at Any EVERY_MONOTONIC
+    \\ first_assum (irule_at Any)
+    \\ simp [FORALL_PROD]
+    \\ rw [EVERY_MEM, LAMBDA_PROD, FORALL_PROD]
+    \\ first_x_assum irule
+    \\ first_assum (irule_at Any)
+    \\ gs [EVERY_MEM, FORALL_PROD, SF SFY_ss])
+  >- ((* Delay *)
+    gs [exp_inv_def, subst_def])
+  >- ((* Box *)
+    gs [exp_inv_def, subst_def])
+  >- ((* Force *)
+    gs [exp_inv_def, subst_def])
+  >- ((* Value *)
+    gs [exp_inv_def, subst_def])
+  >- ((* MkTick *)
+    gs [exp_inv_def, subst_def])
+QED
+
 Theorem exp_rel_eval_to:
   ∀k x y.
     exp_rel x y ∧
+    exp_inv x ∧
     eval_to k x ≠ INL Type_error ⇒
-      ∃j. ($= +++ v_rel) (eval_to k x) (eval_to (k + j) y)
+      ∃j. ($= +++ (λv w. v_rel v w ∧ v_inv v))
+            (eval_to k x)
+            (eval_to (k + j) y)
 Proof
   ho_match_mp_tac eval_to_ind \\ rw []
   \\ qpat_x_assum ‘exp_rel _ _’ mp_tac
   >- ((* Value *)
     rw [Once exp_rel_cases]
-    \\ gs [eval_to_def])
+    \\ gs [eval_to_def, exp_inv_def]
+    \\ rw [Once exp_rel_cases])
   >- ((* Var *)
     rw [Once exp_rel_cases]
     \\ gs [eval_to_def])
   >- ((* App *)
     rename1 ‘App x1 y1’
     \\ rw [Once exp_rel_cases]
+    \\ gs [exp_inv_def]
     \\ rename1 ‘exp_rel x1 x2’
     \\ rename1 ‘exp_rel y1 y2’
     \\ rw [eval_to_def]
@@ -299,18 +485,23 @@ Proof
       \\ gs []
       \\ qpat_assum ‘_ = INL Diverge’ (SUBST1_TAC o SYM)
       \\ first_x_assum (irule_at Any) \\ simp []
-      \\ irule exp_rel_subst
+      \\ irule_at Any exp_rel_subst
+      \\ irule_at Any exp_inv_subst
       \\ qpat_x_assum ‘v_rel v1 u1’ mp_tac
-      \\ simp [Once exp_rel_cases] \\ strip_tac
-      \\ gvs [dest_anyClosure_def]
+      \\ simp [Once exp_rel_cases] \\ strip_tac \\ gvs [dest_anyClosure_def,
+                                                        v_inv_def]
       \\ drule_then (qspec_then ‘n’ assume_tac) LIST_REL_OPTREL
       \\ gs [OPTREL_def]
       \\ qpat_x_assum ‘exp_rel x0 _’ mp_tac
       \\ simp [Once exp_rel_cases] \\ strip_tac \\ gvs []
       \\ simp [MAP_MAP_o, LAMBDA_PROD, combinTheory.o_DEF, GSYM FST_THM,
-               EVERY2_MAP, Once exp_rel_cases]
+               EVERY2_MAP, Once exp_rel_cases, EVERY_MAP, v_inv_def]
       \\ irule_at Any LIST_EQ
-      \\ gvs [LIST_REL_EL_EQN, EL_MAP, ELIM_UNCURRY])
+      \\ gvs [LIST_REL_EL_EQN, EL_MAP, ELIM_UNCURRY]
+      \\ drule_then strip_assume_tac ALOOKUP_SOME_REVERSE_EL
+      \\ gvs [EVERY_EL, EL_MAP]
+      \\ last_x_assum (drule_then assume_tac)
+      \\ gs [exp_inv_def])
     \\ ‘∀j. eval_to (j + j1 + j2 + k) y2 = eval_to (j2 + k) y2’
       by (strip_tac
           \\ irule eval_to_subst_mono \\ gs []
@@ -331,45 +522,53 @@ Proof
           \\ qpat_x_assum ‘exp_rel x0 _’ mp_tac
           \\ rw [Once exp_rel_cases] \\ gs [])
     \\ rename1 ‘v_rel v2 u2’ \\ gs []
-    \\ qsuff_tac ‘exp_rel (subst (w1 ++ [s1,v2]) z1) (subst (w2 ++ [s2,u2]) z2)’
-    >- (
-      strip_tac
-      \\ first_x_assum drule
-      \\ impl_tac
-      >- (
-        strip_tac \\ gs [eval_to_def])
-      \\ disch_then (qx_choose_then ‘j3’ assume_tac)
-      \\ ‘eval_to (j3 + k - 1) (subst (w2 ++ [s2,u2]) z2) ≠ INL Diverge’
-        by (strip_tac
-            \\ Cases_on ‘eval_to (k - 1) (subst (w1 ++ [s1,v2]) z1)’ \\ gs [])
-      \\ drule_then
-        (qspec_then ‘j1 + j2 + j3 + k - 1’ assume_tac) eval_to_subst_mono
-      \\ qexists_tac ‘j3’ \\ gs [])
-    \\ irule exp_rel_subst
+    \\ ‘exp_rel (subst (w1 ++ [s1,v2]) z1) (subst (w2 ++ [s2,u2]) z2) ∧
+        exp_inv (subst (w1 ++ [s1,v2]) z1)’
+      suffices_by
+        (strip_tac
+         \\ first_x_assum drule
+         \\ impl_tac
+         >- (
+           strip_tac \\ gs [eval_to_def])
+         \\ disch_then (qx_choose_then ‘j3’ assume_tac)
+         \\ ‘eval_to (j3 + k - 1) (subst (w2 ++ [s2,u2]) z2) ≠ INL Diverge’
+           by (strip_tac
+               \\ Cases_on ‘eval_to (k - 1) (subst (w1 ++ [s1,v2]) z1)’
+               \\ gs [])
+         \\ drule_then
+           (qspec_then ‘j1 + j2 + j3 + k - 1’ assume_tac) eval_to_subst_mono
+         \\ qexists_tac ‘j3’ \\ gs [])
+    \\ irule_at Any exp_rel_subst
+    \\ irule_at Any exp_inv_subst
     \\ qpat_x_assum ‘v_rel v1 u1’ mp_tac
-    \\ simp [Once exp_rel_cases] \\ strip_tac \\ gvs [dest_anyClosure_def]
+    \\ simp [Once exp_rel_cases] \\ strip_tac \\ gvs [dest_anyClosure_def,
+                                                      v_inv_def]
     \\ drule_then (qspec_then ‘n’ assume_tac) LIST_REL_OPTREL
     \\ gs [OPTREL_def]
     \\ qpat_x_assum ‘exp_rel x0 _’ mp_tac
     \\ simp [Once exp_rel_cases] \\ strip_tac \\ gvs []
     \\ simp [MAP_MAP_o, LAMBDA_PROD, combinTheory.o_DEF, GSYM FST_THM,
-             EVERY2_MAP, Once exp_rel_cases]
+             EVERY2_MAP, EVERY_MAP, Once exp_rel_cases, v_inv_def]
     \\ irule_at Any LIST_EQ
-    \\ gvs [LIST_REL_EL_EQN, EL_MAP, ELIM_UNCURRY])
+    \\ gvs [LIST_REL_EL_EQN, EL_MAP, ELIM_UNCURRY]
+    \\ drule_then strip_assume_tac ALOOKUP_SOME_REVERSE_EL
+    \\ gs [EVERY_EL, EL_MAP]
+    \\ last_x_assum (drule_then assume_tac)
+    \\ gs [exp_inv_def])
   >- ((* Lam *)
     rw [Once exp_rel_cases]
-    \\ simp [eval_to_def]
-    \\ rw [Once exp_rel_cases])
+    \\ gs [eval_to_def, exp_inv_def]
+    \\ rw [Once exp_rel_cases, v_inv_def])
   >- ((* Let NONE *)
-    rw [Once exp_rel_cases]
-    \\ simp [eval_to_def]
-    \\ rename1 ‘Let NONE x1 x2’
+    rename1 ‘Let NONE x1 x2’
+    \\ rw [Once exp_rel_cases]
+    \\ gs [eval_to_def, exp_inv_def]
     \\ IF_CASES_TAC \\ gs []
     >- (
       qexists_tac ‘0’
       \\ simp [])
     \\ ‘eval_to (k - 1) x1 ≠ INL Type_error’
-      by (strip_tac \\ gvs [eval_to_def])
+      by (strip_tac \\ gs [])
     \\ first_x_assum (drule_all_then (qx_choose_then ‘j1’ assume_tac))
     \\ Cases_on ‘eval_to (k - 1) x1 = INL Diverge’ \\ gs []
     >- (
@@ -416,9 +615,9 @@ Proof
     \\ qexists_tac ‘j1 + j2’ \\ gs []
     \\ Cases_on ‘eval_to (j1 + k - 1) y1’ \\ gs [])
   >- ((* Let SOME *)
-    rw [Once exp_rel_cases]
-    \\ simp [eval_to_def]
-    \\ rename1 ‘Let (SOME n) x1 x2’
+    rename1 ‘Let (SOME n) x1 x2’
+    \\ rw [Once exp_rel_cases]
+    \\ gs [eval_to_def, exp_inv_def]
     \\ IF_CASES_TAC \\ gs []
     >- (
       qexists_tac ‘0’
@@ -445,6 +644,8 @@ Proof
     \\ gs []
     \\ ‘exp_rel (subst1 n v1 x2) (subst1 n u1 y2)’
       by (irule exp_rel_subst \\ gs [])
+    \\ ‘exp_inv (subst1 n v1 x2)’
+      by (irule exp_inv_subst \\ gs [])
     \\ first_x_assum (drule_all_then (qx_choose_then ‘j2’ assume_tac))
     \\ Cases_on ‘eval_to (k - 1) (subst1 n v1 x2) = INL Diverge’ \\ gs []
     >- (
@@ -487,21 +688,21 @@ Proof
     cheat)
   >- ((* Delay *)
     rw [Once exp_rel_cases]
-    \\ simp [eval_to_def, Once exp_rel_cases])
+    \\ gs [eval_to_def, v_inv_def, exp_inv_def]
+    \\ rw [Once exp_rel_cases])
   >- ((* Box *)
-    rw [Once exp_rel_cases]
-    \\ gs [eval_to_def]
+    rw [Once exp_rel_cases] \\ gs [eval_to_def, exp_inv_def]
     \\ rename1 ‘exp_rel x y’
     \\ ‘eval_to k x ≠ INL Type_error’
       by (strip_tac \\ gs [])
     \\ first_x_assum (drule_all_then (qx_choose_then ‘j1’ assume_tac))
     \\ qexists_tac ‘j1’
     \\ Cases_on ‘eval_to k x’ \\ Cases_on ‘eval_to (j1 + k) y’ \\ gs []
-    \\ rw [Once exp_rel_cases])
+    \\ rw [Once exp_rel_cases, v_inv_def])
   >- ((* Force *)
     rw [Once exp_rel_cases]
     \\ rename1 ‘exp_rel x y’
-    \\ gs [Once eval_to_def]
+    \\ gs [Once eval_to_def, exp_inv_def]
     \\ ‘eval_to k x ≠ INL Type_error’
       by (strip_tac \\ gs [])
     \\ simp [Once eval_to_def]
@@ -541,7 +742,7 @@ Proof
       >- (
         qexists_tac ‘j1’
         \\ qpat_x_assum ‘v_rel v1 u1’ mp_tac
-        \\ rw [Once exp_rel_cases] \\ gvs [dest_anyThunk_def]
+        \\ rw [Once exp_rel_cases] \\ gvs [dest_anyThunk_def, v_inv_def]
         \\ drule_then (qspec_then ‘n’ assume_tac) LIST_REL_OPTREL
         \\ gs [OPTREL_def]
         \\ qpat_x_assum ‘exp_rel x0 _’ mp_tac
@@ -569,21 +770,30 @@ Proof
         \\ qexists_tac ‘0’ \\ simp []
         \\ qpat_x_assum ‘v_rel v1 u1’ mp_tac
         \\ rw [Once exp_rel_cases] \\ gvs [])
-      \\ ‘exp_rel (subst_funs binds z) (subst_funs binds1 z1)’
+      \\ ‘exp_rel (subst_funs binds z) (subst_funs binds1 z1) ∧
+          exp_inv (subst_funs binds z)’
         by (simp [subst_funs_def]
-            \\ irule exp_rel_subst
+            \\ irule_at Any exp_rel_subst
+            \\ irule_at Any exp_inv_subst
             \\ simp [MAP_MAP_o, combinTheory.o_DEF, LAMBDA_PROD, GSYM FST_THM,
-                     EVERY2_MAP, Once (CONJUNCT2 exp_rel_cases)]
+                     EVERY2_MAP, EVERY_MAP, Once (CONJUNCT2 exp_rel_cases),
+                     v_inv_def]
             \\ irule_at Any LIST_EQ
             \\ qpat_x_assum ‘v_rel v1 u1’ mp_tac
-            \\ simp [Once exp_rel_cases] \\ strip_tac \\ gvs [dest_anyThunk_def]
-            \\ gvs [EL_MAP, ELIM_UNCURRY, LIST_REL_EL_EQN, SF CONJ_ss]
+            \\ simp [Once exp_rel_cases] \\ strip_tac
+            \\ gvs [dest_anyThunk_def, v_inv_def, EL_MAP, ELIM_UNCURRY,
+                    LIST_REL_EL_EQN, SF CONJ_ss]
             \\ ‘OPTREL exp_rel (ALOOKUP (REVERSE f) n) (ALOOKUP (REVERSE g) n)’
               by (irule LIST_REL_OPTREL
                   \\ gvs [CaseEqs ["option", "exp"], LIST_REL_EL_EQN,
                           ELIM_UNCURRY])
             \\ gs [OPTREL_def]
-            \\ gvs [CaseEqs ["option", "exp"], Once exp_rel_cases])
+            \\ gvs [CaseEqs ["option", "exp"], Once exp_rel_cases]
+            \\ Cases_on ‘binds = []’ \\ gs []
+            \\ drule_then strip_assume_tac ALOOKUP_SOME_REVERSE_EL
+            \\ gs [EVERY_EL] \\ rw []
+            \\ last_x_assum (drule_then assume_tac)
+            \\ gs [EL_MAP, exp_inv_def])
       \\ first_x_assum (drule_all_then (qx_choose_then ‘j2’ assume_tac))
       \\ Cases_on ‘eval_to (k - 1) (subst_funs binds z) = INL Diverge’ \\ gs []
       >- (
@@ -614,11 +824,45 @@ Proof
     \\ simp [Once exp_rel_cases] \\ strip_tac \\ gs []
     \\ rename1 ‘v_rel v1 u1’
     \\ IF_CASES_TAC \\ gs []
-    >- cheat (* TODO doesn't work: need thunk in the RHS before diverging *)
+    >- (
+      gs [v_inv_def]
+      \\ simp [Once eval_to_def]
+      \\ Cases_on ‘eval_to 0 y = INL Diverge’ \\ gs []
+      >- (
+        qexists_tac ‘0’
+        \\ simp [])
+      \\ ‘∀j. eval_to j y = eval_to j1 y’
+        by (qx_gen_tac ‘j’
+            \\ drule_then (qspec_then ‘j’ assume_tac) eval_to_subst_mono
+            \\ drule_then (qspec_then ‘j1’ assume_tac) eval_to_subst_mono
+            \\ gs [])
+      \\ simp []
+      \\ drule_then assume_tac v_rel_dest_Tick \\ gs []
+      \\ ‘ISR (dest_anyThunk u1)’
+        by (qpat_x_assum ‘v_rel v1 u1’ mp_tac
+            \\ rw [Once exp_rel_cases] \\ gvs [dest_anyThunk_def, v_inv_def]
+            \\ drule_then (qspec_then ‘n’ assume_tac) LIST_REL_OPTREL
+            \\ gs [OPTREL_def]
+            \\ qpat_x_assum ‘exp_rel x0 _’ mp_tac
+            \\ rw [Once exp_rel_cases] \\ gs [])
+      \\ Cases_on ‘dest_anyThunk u1’ \\ gs []
+      \\ pairarg_tac \\ gvs []
+      \\ qexists_tac ‘0’ \\ simp []
+      \\ qpat_x_assum ‘v_rel v1 _’ mp_tac
+      \\ rw [Once exp_rel_cases] \\ gvs [dest_anyThunk_def, v_inv_def]
+      \\ drule_then (qspec_then ‘n’ assume_tac) LIST_REL_OPTREL
+      \\ gs [OPTREL_def]
+      \\ qpat_x_assum ‘exp_rel x0 _’ mp_tac
+      \\ rw [Once exp_rel_cases] \\ gvs [])
+    \\ drule_then assume_tac v_rel_dest_Tick
+    \\ last_x_assum (qspec_then ‘Atom foo’ assume_tac) \\ gs [](* TODO *)
+    \\ first_assum (qspec_then ‘[]’ mp_tac o CONV_RULE SWAP_FORALL_CONV)
+    \\ simp_tac std_ss [subst_funs_def] \\ simp []
+    \\ disch_then (drule_at (Pos last))
     \\ cheat)
   >- ((* MkTick *)
     rw [Once exp_rel_cases]
-    \\ gs [Once eval_to_def]
+    \\ gs [Once eval_to_def, exp_inv_def]
     \\ simp [Once eval_to_def]
     \\ rename1 ‘exp_rel x y’
     \\ ‘eval_to k x ≠ INL Type_error’
@@ -630,15 +874,17 @@ Proof
       \\ simp [Once eval_to_def])
     \\ qexists_tac ‘j1’
     \\ Cases_on ‘eval_to k x’ \\ Cases_on ‘eval_to (j1 + k) y’ \\ gs []
-    \\ rw [Once exp_rel_cases])
+    \\ rw [Once exp_rel_cases, v_inv_def]
+    \\ cheat (* TODO this needs to be checked in the semantics for MkTick *))
   >- ((* Prim *)
     cheat)
 QED
 
 Theorem exp_rel_eval:
   exp_rel x y ∧
+  exp_inv x ∧
   eval x ≠ INL Type_error ⇒
-    ($= +++ v_rel) (eval x) (eval y)
+    ($= +++ (λv w. v_rel v w ∧ v_inv v)) (eval x) (eval y)
 Proof
   simp [eval_def]
   \\ DEEP_INTRO_TAC some_intro
